\begin{sepproof}{Proof of correctness for algorithm \texttt{fcfs}} \ \\
  We will first show that at the end of the execution, $i \leq n+1$. Suppose that $i > n+1$ on line~\ref{fcfs:return}. This
  means that $F_{cur,n}$ exists and $F_{cur,n} = F - \sum\limits_{i=1}^{n}x_i = 0 \leq F - V$ since, according to the
  condition on line~\ref{fcfs:ifinputvalid}, $F - V \geq 0$. This means however that the \texttt{while} loop on
  line~\ref{fcfs:loop} will break, thus $F_{cur,n+1}$ cannot exist and $i = n + 1$ on line~\ref{fcfs:return}, which is a
  contradiction, thus the first proposition holds. We can also note that, even if $i = n + 1$ at the end of the execution,
  the \texttt{while} loop will break right after the last incrementation, thus the algorithm will never try to read or
  write the nonexistent objects $x_{n+1}, c'_{n+1}$.

  We will now show that $\forall i \in [n], c'_i \leq x_i$, as per the requirement (\ref{naive:req1}). Let $i \in [n]$.
  In line~\ref{fcfs:capinit} we can see that $c'_i = x_i$ and the only other occurence of $c'_i$ is in
  line~\ref{fcfs:setcap} where it is never increased $\left(reduce \geq 0\right)$, thus we see that the requirement
  (\ref{naive:req1}) is satisfied.

  We will finally show that $\sum\limits_{i=1}^{n}c'_i = F - V$. From line~\ref{fcfs:finit} we see that $F_{cur,0} = F$.
  Let $i \in [n]$ such that $F_{cur, i}$ exists. If $F_{cur, i} \leq F - V$, then $F_{cur,i+1}$ does not exist because the
  \texttt{while} loop (line~\ref{fcfs:loop}) breaks after calculating $F_{cur,i}$. Else
  \begin{equation*}
    F_{cur,i+1} = F_{cur,i} - \min{\left(x_{i+1}, F_{cur,i} - F + V\right)} \enspace.
    \mbox{ (lines~\ref{fcfs:setreduce}-~\ref{fcfs:setfcur})}
  \end{equation*}
  If $\nexists i \in [n]: \min{\left(x_i, F_{cur, i-1} - \left(F - V\right)\right)} = F_{cur,i-1} - \left(F - V\right)$,
  then $\forall i \in [n], \min{\left(x_i, F_{cur, i} - \left(F - V\right)\right)} = x_i$, thus from line~\ref{fcfs:setcap}
  it will be $\forall i \in [n], c'_i = 0$ and from line~\ref{fcfs:setfcur}, $F_{cur, n} = 0$. However, we have
  \begin{equation*}
  \begin{gathered}
  \begin{rcases}
    min\left(x_n, F_{cur, n-1} - \left(F - V\right)\right) \neq F_{cur, n-1} - \left(F - V\right) \\
    F_{cur, n-1} = x_n
  \end{rcases} \Rightarrow \\
  \Rightarrow x_n < x_n - \left(F - V\right) \Rightarrow F < V
  \end{gathered}
  \end{equation*}
  which is a contradiction, since if this were the case the algorithm would have failed on lines~\ref{fcfs:ifinputvalid}
  -~\ref{fcfs:inputinvalid}. Thus
  \begin{equation*}
    \exists i \in [n]: \min{\left(x_{i+1}, F_{cur, i} - \left(F - V\right)\right)} = F_{cur,i} - \left(F - V\right)
  \end{equation*}
  That is the only $i \in [n]$ such that $F_{cur,i+1} = F - V$, so
  \begin{equation*}
    \forall 0 < k < i, F_{cur,k} = F_{cur,k-1} - x_k \Rightarrow F_{cur,i} = F - \sum\limits_{k=1}^{i-1}x_k \enspace.
  \end{equation*}
  Furthermore, since $F_{cur,i+1} = F - V$, it is
  \begin{equation*}
  \begin{gathered}
    c'_{i+1} = x_{i+1} - F_{cur,i} + F - V = x_i - F + \sum\limits_{k=1}^{i-1}x_k + F - V \Rightarrow \\
    \Rightarrow c'_{i+1} = \sum\limits_{k=1}^{i}x_k - V \enspace, \\
    \forall k \leq i, c_k' = 0 \mbox{ and} \\
    \forall k > i+1, c_k' = x_k \enspace.
  \end{gathered}
  \end{equation*}
  In total, we have
  \begin{equation*}
    \sum\limits_{k=1}^{n}c_k' = \sum\limits_{k=1}^{i}x_k - V + \sum\limits_{k=i+1}^{n}x_k =
  \sum\limits_{k=1}^{n}x_k - V \Rightarrow \sum\limits_{k=1}^{n}c_k' = F - V \enspace.
  \end{equation*}
  Thus the requirement (\ref{naive:req2}) is satisfied.
\end{sepproof}
