\begin{proof}[Proof of correctness for algorithm \ref{abs}]
   \begin{itemize}
      \item We will show that $\forall i \in [n] \: u_i' \leq x_i$. \\
      On line~\ref{abscapinit}, $\forall i \in [n] \: u_i' = x_i$. Subsequently $u_i'$ is modified on
      line~\ref{abscapzero}, where it becomes equal to 0 and on line~\ref{abscapreduce}, where it is assigned
      $x_i - reduce$. It holds that $x_i - reduce \leq x_i$ because initially $reduce = \frac{V}{n} \geq 0$ and
      subsequently $reduce$ is modified only on line~\ref{absreducemodify} where it is increased ($n > empty$ because of
      line~\ref{absifemptylessn} and $reduce > x_i$ because of line~\ref{absifflowlessreduce}, thus
      $\frac{reduce - x_i}{n - empty} > 0$). We see that $\forall i \in [n], u_i' \leq x_i$.
      \item We will show that $\sum\limits_{i=1}^{n}u_i' = F - V$. \\
      The variable $reduction$ keeps track of the total reduction that has happened and breaks the \textbf{while} loop
      when $reduction \geq V$. We will first show that $reduction = \sum\limits_{i=1}^{n}(x_i- u_i')$ at all times and
      then we will prove that $reduction = V$ at the end of the execution. Thus we will have proven that
      $\sum\limits_{i=1}^{n}u_i'= \sum\limits_{i=1}^{n}x_i - V = F - V$.
      \begin{itemize}
         \item On line~\ref{abscapinit}, $u_i' = x_i \Rightarrow \sum\limits_{i=1}^{n}(x_i- u_i') = 0$ and
         $reduction = 0$. \\
         On line~\ref{abscapzero}, $u_i'$ is reduced to 0 thus $\sum\limits_{i=1}^{n}(x_i- u_i')$ is increased by $u_i'$.
         Similarly, on line~\ref{absreductionincrease} $reduction$ is increased by $u_i'$, the same as the increase in
         $\sum\limits_{i=1}^{n}(x_i- u_i')$. \\
         On line~\ref{abscapreduce}, $u_i'$ is reduced by $u_i' - x_i + reduce$ thus $\sum\limits_{i=1}^{n}(x_i- u_i')$
         is increased by $u_i' - x_i + reduce$. On line~\ref{absreductionmodify}, $reduction$ is increased by
         $u_i' - x_i + reduce$, which is equal to the increase in $\sum\limits_{i=1}^{n}(x_i- u_i')$. \\
         We also have to note that neither $u_i'$ nor $reduction$ is modified in any other way from line~\ref{absloop}
         and on, thus we conclude that $reduction = \sum\limits_{i=1}^{n}(x_i- u_i')$ at all times.
         \item Suppose that $reduction_j > V$ on the line~\ref{absreturn}. Since $reduction_j$ exists, $reduction_{j-1} < V$.
         If $x_{j \: mod \: n} < reduce_{j-1}$ then $reduction_j = reduction_{j-1} + u_{j \: mod \:n}'$.
         Since $reduction_j > V$, $u_{j \: mod \:n}' > V - reduction_{j-1}$. TOCOMPLETE\\

      \end{itemize}
   \end{itemize}
\end{proof}
