\begin{proof}
   Since $\forall i \in [n],c'_i \leq x_i$, by applying the Saturation theorem (\ref{saturation}) we see that $x_i' = c_i'$,
   thus $\delta_i = c_i - x_i'$ and $\Delta_i = x_i - x'_i$. We know that $\sum\limits_{i=1}^{n}x_i' = F - V$, so we have
   \begin{align*}
      ||\delta_i||_1 = \sum\limits_{i=1}^{n}\delta_i &= \sum\limits_{i=1}^{n}\left(c_i - x_i'\right) =
      \sum\limits_{i=1}^{n}c_i - F + V \mbox{ and} \\
      ||\Delta_i||_1 = \sum\limits_{i=1}^{n}\Delta_i &= \sum\limits_{i=1}^{n}\left(x_i - x_i'\right) =
      \sum\limits_{i=1}^{n}x_i - F + V \enspace.
   \end{align*}
   thus $||\delta_i||_1, ||\Delta_i||_1$ are independent from $x_i'$ and $c_i'$.
\end{proof}
