\begin{proof}[Proof of correctness for algorithm \ref{prop}]
   \begin{itemize}
      \item We will show that $\forall i \in [n] \: u_i' \leq x_i$. \\
      According to line~\ref{propcapmodify}, which is the only line where $u_i'$ is changed,
      $u_i' = x_i - \frac{V}{F}x_i \leq x_i$ since $x_i, V, F > 0$ and $V \leq F$.
      \item We will show that $\sum\limits_{i=1}^{n}u_i' = F - V$. \\
      With $F = \sum\limits_{i=1}^{n}x_i$, on line~\ref{propreturn} it holds that $\sum\limits_{i=1}^{n}u_i' =
      \sum\limits_{i=1}^{n}(x_i - \frac{V}{F}x_i) = \sum\limits_{i=1}^{n}x_i - \frac{V}{F}\sum\limits_{i=1}^{n}x_i =
      F - V$.
   \end{itemize}
\end{proof}
